Almost proof of Sinz, def of Sinz k

src/cardinality/sinz_amo.lean
@@ -29,226 +29,684 @@ open assignment
 open encoding
 open distinct
 open gensym
+open amo
 
-variables {l : list (literal V)} {lit lit₁ lit₂ : literal V} {g : gensym V}
+-- NOTES: Proofs need to be cleaned up
+--        Lemmas? The theorem length_lt_length_cons may be useful
+
+variables {l : list (literal V)} {lit l₁ l₂ : literal V} {g : gensym V}
           {τ : assignment V} (hdis : disjoint g.stock (clause.vars l))
+          {c : clause V}
 
 lemma disjoint_fresh_of_disjoint : disjoint g.stock (clause.vars (lit :: l)) → 
-  disjoint (g.fresh.2.stock) (clause.vars l) :=
+  disjoint g.fresh.2.stock (clause.vars l) :=
 begin
-  sorry
+  intro hdis,
+  apply set.disjoint_right.mpr,
+  intros v hv,
+  have := (vars_subset_of_vars_cons lit l) hv,
+  have := set.disjoint_right.mp hdis this,
+  exact set.not_mem_subset (fresh_stock_subset g) this
 end
 
-def sinz_helper : Π (l : list (literal V)), Π (g : gensym V),
+lemma disjoint_fresh_of_disjoint_of_subset {l₂ : list (literal V)} : 
+  disjoint g.stock (clause.vars l) → l₂ ⊆ l → disjoint g.fresh.2.stock (clause.vars l₂) :=
+begin
+  intros hdis hss,
+  apply set.disjoint_right.mpr,
+  intros v hv,
+  have := (clause.vars_subset_of_subset hss) hv,
+  have := set.disjoint_right.mp hdis this,
+  exact set.not_mem_subset (fresh_stock_subset g) this
+end
+
+-- NOTE: Only well-defined for lists with lengths ≥ 2
+def sinz : Π (l : list (literal V)), Π (g : gensym V),
   (disjoint g.stock (clause.vars l)) → cnf V
 | []               _ _            := []
-| [l₁]             g hdis         := [[l₁.flip, Pos (g.fresh.1)]]
+| [l₁]             g hdis         := [] --[[l₁.flip, Pos (g.fresh.1)]] -- may be unneeded
 | (l₁ :: l₂ :: ls) g hdis         := 
     [l₁.flip, Pos (g.fresh.1)] :: 
     [Neg g.fresh.1, Pos g.fresh.2.fresh.1] ::
     [Neg g.fresh.1, l₂.flip] ::
-    (sinz_helper (l₂ :: ls) g.fresh.2 (disjoint_fresh_of_disjoint hdis))
+    (sinz (l₂ :: ls) g.fresh.2 (disjoint_fresh_of_disjoint hdis))
 
-def sinz : Π (l : list (literal V)), Π (g : gensym V),
-  (disjoint g.stock (clause.vars l)) → cnf V
-| []   _ _    := []
-| [l₁] _ _    := []
-| l    g hdis := sinz_helper l g hdis
-
--- TODO: helper and sinz or one function and just prove theorems for lists of
--- at least 2 elements?
-
-/-
-def sinz_alt2 : Π (l : list (literal V)), Π (g : gensym V),
-  (disjoint g.stock (clause.vars l)) → cnf V
-| []   _ _    := []
-| [l₁] _ _    := []
-| l    g hdis := (foldr (++) [] (map (λ (p : (nat × literal V)), 
-                  if p.1 = length l - 1 then [[p.2]] else [[p.2]]) (enum l)))
--/
-
-/-
-lemma eval_tt_cons_of_eval_tt_of_neg (hdis : disjoint g.stock (clause.vars (lit :: l))) : 
-  (sinz_helper l g.fresh.2 (disjoint_fresh_of_disjoint hdis) [g.fresh.1])
-  -/
-
--- Really an iff relation, but one way is fine for now?
-theorem exists_signal_mem_of_mem_of_length_ge_two : length l ≥ 2 → lit ∈ l → 
-  ∃ {s : V}, s ∈ g.stock ∧ [lit.flip, Pos s] ∈ sinz l g hdis :=
+theorem mem_sinz_vars_of_mem : length l ≥ 2 → clause.vars l ⊆ cnf.vars (sinz l g hdis) :=
 begin
-  intros hl hmem,
-  induction l with l₁ ls ih generalizing g,
-  { exact absurd hmem (not_mem_nil _) },
-  { cases ls with l₂ ls,
-    { simp [length] at hl, linarith },
-    { rcases eq_or_mem_of_mem_cons hmem with (rfl | h),
-      { use g.fresh.1,
-        rw [sinz, sinz_helper],
-        exact ⟨fresh_mem_stock g, mem_cons_self _ _⟩ },
-      { cases ls with l₃ ls,
-        { simp at h,
-          use g.fresh.2.fresh.1,
-          split, { exact fresh_fresh_mem_stock g },
-          rw [sinz, sinz_helper, sinz_helper],
-          simp [h] },
-        { have : length (l₂ :: l₃ :: ls) ≥ 2,
-          { simp, linarith },
-          rcases ih this h (disjoint_fresh_of_disjoint hdis) with ⟨s, hs, hc⟩,
-          rw sinz at hc |-,
-          rw sinz_helper,
-          use s, split,
-          { exact fresh_stock_subset g hs },
-          { simp [hc] } } } } }
+  intro hlen,
+  induction l using strong_induction_on_lists with l ih generalizing g,
+  rcases exists_cons_cons_of_length_ge_two hlen with ⟨l₁, l₂, ls, rfl⟩,
+  intros v hv,
+  rw sinz,
+  simp [clause.vars] at hv,
+  rcases hv with (rfl | rfl | hv),
+  { simp [cnf.vars, clause.vars, flip_var_eq] },
+  { simp [cnf.vars, clause.vars, flip_var_eq] },
+  { cases ls with l₃ ls,
+    { rw clause.vars_nil at hv,
+      exact absurd hv (finset.not_mem_empty _) },
+    { have hlen' : length (l₂ :: l₃ :: ls) ≥ 2, dec_trivial,
+      have hless : length (l₂ :: l₃ :: ls) < length (l₁ :: l₂ :: l₃ :: ls), simp,
+      have hdis' := disjoint_fresh_of_disjoint hdis,
+      simp [cnf.vars],
+      right, right, right,
+      exact (ih _ hless hlen' hdis') (vars_subset_of_vars_cons l₂ (l₃ :: ls) hv) } }
 end
 
-theorem all_ff_eval_tt : length l ≥ 2 → (sinz_helper l g hdis).eval all_ff = tt :=
-begin
-  induction l with l₁ ls ih,
-  { intro hlen, rw length at hlen, linarith },
-  { intro hlen,
-    cases ls with l₂ ls,
-    { simp [length] at hlen, linarith},
-    { cases ls with l₃ ls,
-      {
-        simp [eval_tt_iff_forall_clause_eval_tt, sinz_helper],
-      } 
-    }
-  }
-end
-
-theorem ne_of_distinct_of_length_ge_two {s₁ s₂ : V} : length l ≥ 2 → distinct lit₁ lit₂ l →
-  s₁ ∈ g.stock → s₂ ∈ g.stock → [lit₁.flip, Pos s₁] ∈ sinz l g hdis →
-  [lit₂.flip, Pos s₂] ∈ sinz l g hdis → s₁ ≠ s₂ :=
-begin
-  intros hl hd hs₁ hs₂ hmem₁ hmem₂,
-  induction l with l₁ ls ih,
-  { exact absurd hd (not_distinct_nil _ _) },
-  { cases ls with l₂ ls,
-    { exact absurd hd (not_distinct_singleton _ _ _) },
-    { cases ls with l₃ ls,
-      { 
-
-      }
-
-    }
-  }
-end
-
-lemma eval_tt_iff_distinct_eval_ff_of_eval_tt :
-  (sinz l g hdis).eval τ = tt ↔ (∀ {lit₁ lit₂ : literal V},
-  distinct lit₁ lit₂ l → lit₁.eval τ = tt → lit₂.eval τ = ff) :=
-begin
-  induction l with l₁ ls ih generalizing g,
-  { split,
-    { intros _ lit₁ lit₂ hd, exact absurd hd (not_distinct_nil _ _) },
-    { rw [sinz, cnf.eval_nil], tautology } },
-  { cases ls with l₂ ls,
-    { split,
-      { intros _ lit₁ lit₂ hd, exact absurd hd (not_distinct_singleton _ _ _) },
-      { rw [sinz, cnf.eval_nil], tautology } },
-    { split,
-      {
-        intros heval lit₁ lit₂ hd h₁,
-        sorry,
-      },
-      {
-        sorry
-      } } }
-end
-
-theorem sinz_encodes_amo {l : list (literal V)} {g : gensym V} (hdis : disjoint g.stock (clause.vars l)) :
-  encodes amo (sinz l g hdis) l :=
+theorem mem_or_mem_of_mem_vars {v : V} : v ∈ cnf.vars (sinz l g hdis) → 
+  v ∈ clause.vars l ∨ v ∈ g.stock :=
 begin
   induction l using strong_induction_on_lists with l ih generalizing g,
-  intro τ,
+  cases l with l₁ ls,
+  { rw [sinz, cnf.vars_nil], intro h, exact absurd h (finset.not_mem_empty _) },
+  cases ls with l₂ ls,
+  { rw [sinz, cnf.vars_nil], intro h, exact absurd h (finset.not_mem_empty _) },
+  rw sinz,
+  intro h,
+  simp [cnf.vars, clause.vars, flip_var_eq, var] at h,
+  rcases h with (rfl | rfl | rfl | rfl | rfl | h),
+  { left, simp [clause.vars] },
+  { exact or.inr (fresh_mem_stock g) },
+  { exact or.inr (fresh_fresh_mem_stock g) },
+  { exact or.inr (fresh_mem_stock g) },
+  { left, simp [clause.vars] },
+  { cases ls with l₃ ls,
+    { rw [sinz, cnf.vars_nil] at h,
+      exact absurd h (finset.not_mem_empty _) },
+    { have hlen := length_lt_length_cons l₁ (l₂ :: l₃ :: ls),
+      have hdis' := disjoint_fresh_of_disjoint hdis,
+      rcases ih _ hlen hdis' h with (hv | hv),
+      { exact or.inl ((vars_subset_of_vars_cons l₁ _) hv) },
+      { exact or.inr (fresh_stock_subset g hv) } } }
+end
+
+theorem not_mem_sinz_vars_of_not_mems {v : V} : v ∉ clause.vars l → 
+  v ∉ g.stock → v ∉ cnf.vars (sinz l g hdis) :=
+begin
+  intros hvar hstock,
+  induction l using strong_induction_on_lists with l ih generalizing g,
+  cases l with l₁ ls,
+  { simp [sinz] },
+  cases ls with l₂ ls,
+  { simp [sinz] },
+  have hg₁ : v ≠ g.fresh.1,
+  { exact (ne_of_mem_of_not_mem (fresh_mem_stock g) hstock).symm },
+  have hg₂ : v ≠ g.fresh.2.fresh.1,
+  { exact (ne_of_mem_of_not_mem (fresh_fresh_mem_stock g) hstock).symm },
+  cases ls with l₃ ls,
+  { simp [clause.vars, not_or_distrib] at hvar,
+    rcases hvar with ⟨hvar₁, hvar₂⟩,
+    simp [sinz, cnf.vars, clause.vars, not_or_distrib, flip_var_eq, var,
+      hvar₁, hvar₂, hg₁, hg₂] },
+  { rw sinz,
+    have hvar' : v ∉ clause.vars (l₂ :: l₃ :: ls),
+    { rw clause.vars at hvar,
+      simp only [not_or_distrib, finset.mem_union, finset.mem_singleton] at hvar,
+      exact hvar.2 },
+    have hless : length (l₂ :: l₃ :: ls) < length (l₁ :: l₂ :: l₃ :: ls), simp,
+    have hdis' := disjoint_fresh_of_disjoint hdis,
+    have : v ∉ g.fresh.2.stock,
+    { intro hcon,
+      exact hstock ((fresh_stock_subset g) hcon) },
+    have ihred := ih _ hless hvar' hdis' this,
+    simp [clause.vars, not_or_distrib] at hvar,
+    rcases hvar with ⟨hvar₁, hvar₂, hvar₃, hvar⟩,
+    simp [cnf.vars, clause.vars, not_or_distrib, flip_var_eq, var,
+      hvar₁, hvar₂, hvar₃, hg₁, hg₂, ihred] }
+end
+
+/-
+theorem sinz_amz : amz.eval τ l = tt → 
+  (sinz l g hdis).eval (assignment.ite (clause.vars l) τ all_ff) = tt :=
+begin
+  induction l using strong_induction_on_lists with l ih generalizing g,
   cases l with l₁ ls,
   { simp [sinz] },
   { cases ls with l₂ ls,
-    { simp [sinz], use τ },
-    { cases ls with l₃ ls,
-      { split,
-        { simp [← amo.eval, sinz, sinz_helper, eval_tt_iff_forall_clause_eval_tt],
-          intro heval,
-          cases h₁ : (literal.eval τ l₁),
-          { use [assignment.ite (clause.vars [l₁, l₂]) τ all_ff],
-            split,
-            {
-              have hmem₁ : l₁.flip.var ∈ clause.vars [l₁, l₂],
-              { simp [flip_var_eq, clause.vars] },
-              have hmem₂ : l₂.flip.var ∈ clause.vars [l₁, l₂],
-              { simp [flip_var_eq, clause.vars] },
-              have hnmem₁ : g.fresh.1 ∉ clause.vars [l₁, l₂],
-              { have := set.disjoint_left.mp hdis (fresh_mem_stock g),
-                assumption }, -- TODO coercion is silly
-              have hnmem₂ : g.fresh.2.fresh.1 ∉ clause.vars [l₁, l₂],
-              { have := fresh_mem_stock g.fresh.2,
-                have := set.disjoint_left.mp hdis (fresh_stock_subset g this),
-                assumption }, -- TODO this too
-              simp [eval_tt_iff_exists_literal_eval_tt, literal.eval],
-              split,
-              { use [l₁.flip],
-                rw ite_pos_lit τ all_ff hmem₁,
-                simp [eval_flip, h₁] },
-              { split,
-                { use [Neg g.fresh.1],
-                  simp [literal.eval],
-                  rw ite_neg τ all_ff hnmem₁,
-                  refl },
-                { split,
-                  { use [Neg g.fresh.1],
-                    simp [literal.eval],
-                    rw ite_neg τ all_ff hnmem₁,
-                    refl },
-                  {
-
-                  }
-
-                }
-
-              }
-            },
-            { exact (ite_eqod τ all_ff (clause.vars [l₁, l₂])).symm }
-          }
-        }
-      },
-      
-      have hlen : length (l₂ :: ls) < length (l₁ :: l₂ :: ls), simp,
-      have ihred := ih (l₂ :: ls) hlen (disjoint_fresh_of_disjoint hdis) τ,
-      split,
-      { intro hamo,
-        rw ← amo.eval at hamo,
-        have := amo.eval_tt_of_eval_tt_cons hamo,
-        rcases ihred.mp this with ⟨σ, heval', heqod'⟩,
-        use assignment.ite (clause.vars (l₁ :: l₂ :: ls)) τ σ,
-        split,
-        {
-          sorry,
-        },
-        { exact (ite_eqod τ σ (clause.vars (l₁ :: l₂ :: ls))).symm } },
-      {
-        rintros ⟨σ, heval, heqod⟩,
-        rw ← amo.eval,
-        rw amo.amo_eval_tt_iff_distinct_eval_ff_of_eval_tt,
-        intros lit₁ lit₂ hd h₁,
-
-        rw eval_tt_iff_forall_clause_eval_tt at heval,
-        rw [sinz, sinz_helper] at heval,
-        simp at heval,
-        rcases heval with ⟨c₁, c₂, c₃, hp⟩,
-        rw [← eval_tt_iff_forall_clause_eval_tt] at hp,
-
-
-        rcases hd with ⟨i, j, hi, hj, hij, hil, hjl⟩,
-        cases i,
-        {
-
-        }
-       -- have := (eval_tt_iff_distinct_eval_ff_of_eval_tt hdis).mp heval,
-
-        --rw [eval_tt_iff_forall_clause_eval_tt, sinz, sinz_helper] at heval,
-        --have : ∃ (σ : assignment V), cnf.eval σ (sinz (l₂ :: ls) g.fresh.2 
-        --  (disjoint_fresh_of_disjoint hdis)) = tt ∧ (τ ≡clause.vars (l₂ :: ls)≡ σ),
-      } } }
+    { simp [sinz] },
+    { intro hamz,
+      have hdis' := disjoint_fresh_of_disjoint hdis,
+      rw [eval_tt_iff_forall_clause_eval_tt, sinz],
+      intros c hc,
+      simp at hc,
+      rw eval_tt_iff_exists_literal_eval_tt,
+      rcases hc with (rfl | rfl | rfl | hc),
+      { use l₁.flip,
+        rw [eval_flip,ite_pos_lit (mem_vars_of_mem (mem_cons_self l₁ _))],
+        rw amz.eval_tt_iff_forall_eval_ff at hamz,
+        simp [hamz l₁ (mem_cons_self l₁ _)] },
+      { use Neg g.fresh.1,
+        have := set.disjoint_left.mp hdis (fresh_mem_stock g), -- TODO why not ellide?
+        simp [literal.eval, ite_neg this, all_ff] },
+      { use Neg g.fresh.1,
+        have := set.disjoint_left.mp hdis (fresh_mem_stock g), -- TODO why not ellide?
+        simp [literal.eval, ite_neg this, all_ff] },
+      { have hlen : length (l₂ :: ls) < length (l₁ :: l₂ :: ls), simp,
+        have := ih (l₂ :: ls) hlen hdis' (amz.eval_tt_of_eval_tt_cons hamz),
+        rw eval_tt_iff_forall_clause_eval_tt at this,
+        rcases eval_tt_iff_exists_literal_eval_tt.mp (this c hc) with ⟨l, hlc, hl⟩,
+        use [l, hlc],
+        by_cases hlmem : (l.var ∈ clause.vars (l₂ :: ls)),
+        { rw ite_pos_lit (vars_subset_of_vars_cons l₁ (l₂ :: ls) hlmem),
+          rw ite_pos_lit hlmem at hl,
+          exact hl },
+        { rw ite_neg_lit hlmem at hl,
+          by_cases h₁ : l₁.var ∈ clause.vars (l₂ :: ls),
+          { have : l.var ∉ clause.vars (l₁ :: l₂ :: ls),
+            { rw clause.vars,
+              intro hcon,
+              rcases finset.mem_union.mp hcon with (hcon | hcon),
+              { simp at hcon,
+                rw ← hcon at h₁,
+                exact hlmem h₁ },
+              { exact hlmem hcon } },
+            rw ite_neg_lit this,
+            exact hl },
+          { have := mem_vars_of_mem (mem_cons_self l₁ (l₂ :: ls)),
+            have := set.disjoint_right.mp hdis this,
+            have := set.not_mem_subset (fresh_stock_subset g) this,
+            have h₁' := not_mem_sinz_vars_of_not_mems hdis' h₁ this,
+            have := clause_vars_subset_of_vars_of_mem hc
+              (mem_vars_of_mem hlc),
+            --have : l.var ≠ l₁.var, library_search,
+            have := ne_of_mem_of_not_mem this h₁',
+            have : l.var ∉ clause.vars (l₁ :: l₂ :: ls),
+            { rw clause.vars,
+              simp [not_or_distrib],
+              exact ⟨this, hlmem⟩ },
+            rw ite_neg_lit this,
+            exact hl } } } } }
 end
+-/
+
+-- NOTE: This theorem and the above are very similar, fixes to one go to other
+theorem sinz_amz' : amz.eval τ l = tt →
+  (sinz l g hdis).eval (assignment.ite (clause.vars l) τ all_tt) = tt :=
+begin
+  induction l using strong_induction_on_lists with l ih generalizing g,
+  cases l with l₁ ls,
+  { simp [sinz] },
+  { cases ls with l₂ ls,
+    { simp [sinz] },
+    { intro hamz,
+      have hdis' := disjoint_fresh_of_disjoint hdis,
+      rw [eval_tt_iff_forall_clause_eval_tt, sinz],
+      intros c hc,
+      simp at hc,
+      rw eval_tt_iff_exists_literal_eval_tt,
+      rcases hc with (rfl | rfl | rfl | hc),
+      { use l₁.flip,
+        rw [eval_flip, ite_pos_lit (mem_vars_of_mem (mem_cons_self l₁ _))],
+        rw amz.eval_tt_iff_forall_eval_ff at hamz,
+        simp [hamz l₁ (mem_cons_self l₁ _)] },
+      { use Pos g.fresh.2.fresh.1,
+        have := set.disjoint_left.mp hdis (fresh_fresh_mem_stock g),
+        simp [literal.eval, ite_neg this, all_tt] },
+      { use l₂.flip,
+        have : l₂.var ∈ clause.vars (l₁ :: l₂ :: ls), simp [clause.vars],
+        rw [eval_flip, ite_pos_lit this],
+        rw amz.eval_tt_iff_forall_eval_ff at hamz,
+        simp [hamz l₂ (mem_cons_of_mem _ (mem_cons_self l₂ _))] },
+      { have hlen : length (l₂ :: ls) < length (l₁ :: l₂ :: ls), simp,
+        have := ih (l₂ :: ls) hlen hdis' (amz.eval_tt_of_eval_tt_cons hamz),
+        rw eval_tt_iff_forall_clause_eval_tt at this,
+        rcases eval_tt_iff_exists_literal_eval_tt.mp (this c hc) with ⟨l, hlc, hl⟩,
+        use [l, hlc],
+        by_cases hlmem : (l.var ∈ clause.vars (l₂ :: ls)),
+        { rw ite_pos_lit (vars_subset_of_vars_cons l₁ (l₂ :: ls) hlmem),
+          rw ite_pos_lit hlmem at hl,
+          exact hl },
+        { rw ite_neg_lit hlmem at hl,
+          by_cases h₁ : l₁.var ∈ clause.vars (l₂ :: ls),
+          { have : l.var ∉ clause.vars (l₁ :: l₂ :: ls),
+            { rw clause.vars,
+              intro hcon,
+              rcases finset.mem_union.mp hcon with (hcon | hcon),
+              { simp at hcon,
+                rw ← hcon at h₁,
+                exact hlmem h₁ },
+              { exact hlmem hcon } },
+            rw ite_neg_lit this,
+            exact hl },
+          { have := mem_vars_of_mem (mem_cons_self l₁ (l₂ :: ls)),
+            have := set.disjoint_right.mp hdis this,
+            have := set.not_mem_subset (fresh_stock_subset g) this,
+            have h₁' := not_mem_sinz_vars_of_not_mems hdis' h₁ this,
+            have := clause_vars_subset_of_vars_of_mem hc
+              (mem_vars_of_mem hlc),
+            --have : l.var ≠ l₁.var, library_search,
+            have := ne_of_mem_of_not_mem this h₁',
+            have : l.var ∉ clause.vars (l₁ :: l₂ :: ls),
+            { rw clause.vars,
+              simp [not_or_distrib],
+              exact ⟨this, hlmem⟩ },
+            rw ite_neg_lit this,
+            exact hl } } } } }
+end
+
+theorem sinz_amo (hdis : disjoint g.stock (clause.vars (l₁ :: l))) : 
+  amz.eval τ l = tt → l₁.eval τ = tt → 
+  (sinz (l₁ :: l) g hdis).eval (assignment.ite (clause.vars (l₁ :: l)) τ all_tt) = tt :=
+begin
+  intros hamz h₁,
+  cases l with l₂ ls,
+  { simp [sinz] },
+  { rw [eval_tt_iff_forall_clause_eval_tt, sinz],
+    intros c hc,
+    simp at hc,
+    rw eval_tt_iff_exists_literal_eval_tt,
+    rcases hc with (rfl | rfl | rfl | hc),
+    { use Pos g.fresh.1,
+      have := set.disjoint_left.mp hdis (fresh_mem_stock g),
+      simp [literal.eval, ite_neg this, all_tt] },
+    { use Pos g.fresh.2.fresh.1,
+      have := set.disjoint_left.mp hdis (fresh_fresh_mem_stock g),
+      simp [literal.eval, ite_neg this, all_tt] },
+    { use l₂.flip,
+      have : l₂.var ∈ clause.vars (l₁ :: l₂ :: ls), simp [clause.vars],
+      rw [eval_flip, ite_pos_lit this],
+      rw amz.eval_tt_iff_forall_eval_ff at hamz,
+      simp [hamz l₂ (mem_cons_self l₂ _)] },
+    {
+      have hdis' := disjoint_fresh_of_disjoint hdis,
+      have := sinz_amz' hdis' hamz,
+      rw eval_tt_iff_forall_clause_eval_tt at this,
+      rcases eval_tt_iff_exists_literal_eval_tt.mp (this c hc) with ⟨l, hlc, hl⟩,
+      use [l, hlc],
+      have := cnf.clause_vars_subset_of_vars_of_mem hc,
+      rcases mem_or_mem_of_mem_vars hdis' (this (mem_vars_of_mem hlc)) with (hv | hv),
+      { rw ite_pos_lit (mem_vars_cons_of_mem_vars l₁ hv),
+        rw ite_pos_lit hv at hl,
+        exact hl },
+      { have := set.disjoint_left.mp hdis (fresh_stock_subset g hv),
+        rw ite_neg_lit this,
+        rw clause.vars at this,
+        simp [not_or_distrib] at this,
+        rw ite_neg_lit this.2 at hl,
+        exact hl } } }
+end
+
+theorem sinz_signal (hdis : disjoint g.stock (clause.vars (l₁ :: l))) :
+  τ g.fresh.1 = tt → (sinz (l₁ :: l) g hdis).eval τ = tt → 
+  ∀ (lit : literal V), lit ∈ l → lit.eval τ = ff :=
+begin
+  sorry,
+  /-
+  intro ht,
+  induction l using strong_induction_on_lists with l ih generalizing g,
+  cases l with l₂ ls,
+  { simp [sinz] },
+  intros heval lit hlit,
+  rw [sinz, eval_tt_iff_forall_clause_eval_tt] at heval,
+  simp at heval,
+  rcases heval with ⟨h₁, h₂, h₃, h₄⟩,
+  have hlen : length ls < length (l₂ :: ls), simp,
+  have hdis' : disjoint g.fresh.2.stock (clause.vars (l₁ :: ls)),
+  {
+    apply set.disjoint_right.mpr,
+    intros v hv,
+    have : clause.vars (l₁ :: ls) ⊆ clause.vars (l₁ :: l₂ :: ls),
+    { apply clause.vars_subset_of_subset,
+      simp [subset_cons_of_subset l₁ (subset_cons l₂ ls)] },
+    have := this hv,
+    have := set.disjoint_right.mp hdis this,
+    intro hcon,
+    exact this (fresh_stock_subset g hcon) },
+    have ihred := ih _ hlen hdis',
+    sorry
+
+   simp [sinz, eval_tt_iff_forall_clause_eval_tt],
+    rintros ht hc₁ hc₂ hc₃ rfl,
+    simp [eval_tt_iff_exists_literal_eval_tt] at hc₃,
+    rcases hc₃ with ⟨l, (rfl | rfl), hl⟩,
+    { rw [literal.eval, ht] at hl, contradiction },
+    { simp [eval_flip] at hl, exact hl } },
+  {
+    intros ht heval,
+    rw [sinz, eval_tt_iff_forall_clause_eval_tt] at heval,
+    simp at heval,
+    have hlen : length (l₃ :: ls) < length (l₂ :: l₃ :: ls), simp,
+    have hdis' := disjoint_fresh_of_disjoint hdis,
+    have ihred := (ih _ hlen hdis'),
+
+  }
+  -/
+end
+
+#exit
+
+theorem sinz_base_case (hdis : disjoint g.stock (clause.vars [l₁, l₂])) : 
+  encodes amo (sinz [l₁, l₂] g hdis) [l₁, l₂] :=
+begin
+  intro τ,
+  split,
+  { intro hamo,
+    cases h₁ : (literal.eval τ l₁),
+    { use assignment.ite (clause.vars [l₁, l₂]) τ all_ff,
+      split,
+      { have hnmem₁ : g.fresh.1 ∉ clause.vars [l₁, l₂],
+        { have := set.disjoint_left.mp hdis (fresh_mem_stock g), assumption },
+        rw eval_tt_iff_forall_clause_eval_tt,
+        intros c hc,
+        simp [sinz] at hc,
+        rw eval_tt_iff_exists_literal_eval_tt,
+        rcases hc with (rfl | rfl | rfl),
+        { use l₁.flip,
+          have hmem₁ : l₁.flip.var ∈ clause.vars [l₁, l₂],
+          { simp [flip_var_eq, clause.vars] },
+          rw [ite_pos_lit hmem₁, eval_flip],
+          simp [h₁] },
+        { use Neg g.fresh.1,
+          simp [literal.eval, ite_neg hnmem₁, all_ff] },
+        { use Neg g.fresh.1,
+          simp [literal.eval, ite_neg hnmem₁, all_ff]
+        } },
+      { exact (ite_eqod _ _ _).symm } },
+    { rw [← amo.eval, eval_cons_pos h₁] at hamo,
+      use [(assignment.ite (clause.vars [l₁, l₂]) τ all_tt),
+        sinz_amo hdis hamo h₁, (ite_eqod _ _ _).symm] } },
+  { rintros ⟨σ, heval, heqod⟩,
+    have heq : literal.eval τ l₂ = literal.eval σ l₂,
+    { have : l₂.var ∈ clause.vars [l₁, l₂],
+      { simp [clause.vars] },
+        exact eval_eq_of_eqod_of_var_mem heqod this },
+      rw [← amo.eval, eval_eq_amo_of_eqod heqod],
+      rw eval_tt_iff_forall_clause_eval_tt at heval,
+      cases h₁ : (literal.eval σ l₁),
+      { rw [eval_cons_neg h₁, amo.eval_singleton] },
+      { have : ∀ (lit₁ lit₂ : literal V), (distinct lit₁ lit₂ [l₁, l₂]) → 
+          lit₁.eval τ = tt → lit₂.eval τ = ff,
+        { intros lit₁ lit₂ hd _,
+          rcases eq_of_distinct_double hd with ⟨rfl, rfl⟩,
+          simp [sinz, clause.eval, eval_flip, literal.eval, h₁] at heval,
+          rcases heval with ⟨hs₁, hs₂, hs₃⟩,
+          simp [hs₁] at hs₃,
+          rw heq,
+          exact hs₃ },
+        rw ← eval_eq_amo_of_eqod heqod,
+        exact amo_eval_tt_iff_distinct_eval_ff_of_eval_tt.mpr this } }
+end
+
+theorem sinz_encodes_amo : encodes amo (sinz l g hdis) l :=
+begin
+  induction l using strong_induction_on_lists with l ih generalizing g,
+  cases l with l₁ ls,
+  { intro τ, simp [sinz] },
+  cases ls with l₂ ls,
+  { intro τ, simp [sinz], use τ },
+
+  have hdis' := disjoint_fresh_of_disjoint hdis,
+
+  cases ls with l₃ ls,
+  { exact sinz_base_case hdis },
+  { intro τ, 
+    have hlen : length (l₂ :: l₃ :: ls) < length (l₁ :: l₂ :: l₃ :: ls), simp,
+    have ihred := (ih _ hlen hdis') τ,
+    split,
+    { intro hamo,
+      cases h₁ : (literal.eval τ l₁),
+      { rcases ihred.mp (eval_tt_of_eval_tt_cons hamo) with ⟨σ, heval', hs⟩,
+        use assignment.ite (cnf.vars (sinz (l₂ :: l₃ :: ls) g.fresh.2 hdis')) σ 
+            (assignment.ite {l₁.var} τ all_ff),
+        have heval₁ : literal.eval (assignment.ite (cnf.vars (sinz (l₂ :: l₃ :: ls) g.fresh.2 hdis')) σ 
+            (assignment.ite {l₁.var} τ all_ff)) l₁ = ff,
+        { by_cases h : (l₁.var ∈ cnf.vars (sinz (l₂ :: l₃ :: ls) g.fresh.2 hdis')),
+          { rw ite_pos_lit h,
+            rcases mem_or_mem_of_mem_vars hdis' h with (hv | hv),
+            { rw ← eval_eq_of_eqod_of_var_mem hs hv,
+              exact h₁ },
+            { have : l₁.var ∈ clause.vars (l₁ :: l₂ :: l₃ :: ls),
+              { rw clause.vars,
+                exact finset.mem_union.mpr (or.inl (finset.mem_singleton_self l₁.var)) },
+              have := set.disjoint_right.mp hdis this,
+              have := (fresh_stock_subset g) hv,
+              contradiction } },
+          { rw ite_neg_lit h,
+            rw ite_pos_lit (finset.mem_singleton_self l₁.var),
+            exact h₁ } },
+        have heval₂ : (assignment.ite (cnf.vars (sinz (l₂ :: l₃ :: ls) g.fresh.2 hdis')) σ 
+            (assignment.ite {l₁.var} τ all_ff)) g.fresh.1 = ff,
+        { 
+          have h₀ := set.disjoint_left.mp hdis (fresh_mem_stock g),
+          have h₁ : g.fresh.1 ∉ clause.vars (l₂ :: l₃ :: ls),
+          { rw clause.vars at h₀,
+            simp [not_or_distrib] at h₀,
+            exact h₀.2 },
+          have h₂ : g.fresh.1 ∉ g.fresh.2.stock,
+          { exact fresh_not_mem_fresh_stock g },
+          rw ite_neg (not_mem_sinz_vars_of_not_mems hdis' h₁ h₂),
+          rw clause.vars at h₀,
+          simp [not_or_distrib] at h₀,
+          have : g.fresh.1 ∉ {l₁.var},
+          { rw finset.mem_singleton,
+            exact h₀.1 },
+          rw [ite_neg this, all_ff] },
+        split,
+        { rw [eval_tt_iff_forall_clause_eval_tt, sinz],
+          intros c hc,
+          rw eval_tt_iff_exists_literal_eval_tt,
+          simp at hc,
+          rcases hc with (rfl | rfl | rfl | hc),
+          { use l₁.flip,
+            simp [eval_flip, heval₁] },
+          { use Neg g.fresh.1,
+            simp [literal.eval, heval₂] },
+          { use Neg g.fresh.1,
+            simp [literal.eval, heval₂] },
+          { rw ← eval_tt_iff_exists_literal_eval_tt,
+            rw eval_tt_iff_forall_clause_eval_tt at heval',
+            rw ← heval' c hc,
+            apply eval_eq_clause_of_eqod,
+            apply eqod_subset (clause_vars_subset_of_vars_of_mem hc),
+            intros v hv,
+            rw ite_pos hv } },
+        { intros v hv,
+          rcases finset.mem_union.mp hv with (hvmem | hvmem),
+          { cases l₁;
+            { simp [literal.flip, literal.eval, var] at h₁ hvmem heval₁ |-,
+              simp [heval₁, hvmem, h₁] } },
+          { have : length (l₂ :: l₃ :: ls) ≥ 2, dec_trivial,
+            rw ite_pos (mem_sinz_vars_of_mem hdis' this hvmem),
+            exact hs v hvmem } } },
+      { rw [← amo.eval, eval_cons_pos h₁] at hamo,
+        use [(assignment.ite (clause.vars (l₁ :: l₂ :: l₃ :: ls)) τ all_tt),
+        sinz_amo hdis hamo h₁, 
+        (ite_eqod (clause.vars (l₁ :: l₂ :: l₃ :: ls)) τ _).symm] } },
+    { rintros ⟨σ, heval, heqod⟩,
+      cases h₁ : (literal.eval τ l₁),
+      { rw [eval_tt_iff_forall_clause_eval_tt, sinz] at heval,
+        simp at heval,
+        rcases heval with ⟨hc₁, hc₂, hc₃, hc₄⟩,
+        rw ← eval_tt_iff_forall_clause_eval_tt at hc₄,
+        rw [← amo.eval, eval_cons_neg h₁],
+        exact ihred.mpr ⟨σ, hc₄, eqod_subset (vars_subset_of_vars_cons _ _) heqod⟩ },
+      { rw [← amo.eval, eval_cons_pos h₁],
+        cases hf : (σ g.fresh.1),
+        { rw [eval_tt_iff_forall_clause_eval_tt] at heval,
+          have : [l₁.flip, Pos (g.fresh.1)] ∈ sinz (l₁ :: l₂ :: l₃ :: ls) g hdis,
+          { exact mem_cons_self _ _ },
+          have := heval _ this,
+          simp [eval_tt_iff_exists_literal_eval_tt] at this,
+          rcases this with ⟨w, (rfl | rfl), hw⟩,
+          { rw [eval_flip, ← h₁] at hw, -- This can be cleaned up
+            have := eval_eq_of_eqod_of_var_mem heqod (mem_vars_of_mem (mem_cons_self l₁ _)),
+            rw h₁ at this,
+            simp [← this] at hw,
+            rw ← hw at h₁,
+            contradiction },
+          { rw [literal.eval, hf] at hw,
+            contradiction } },
+        { rw amz.eval_eq_amz_of_eqod (eqod_subset (vars_subset_of_vars_cons l₁ (l₂ :: l₃ :: ls)) heqod),
+          exact amz.eval_tt_iff_forall_eval_ff.mpr (sinz_signal hdis hf heval) } } } }
+end
+
+/-
+theorem sinz_encodes_amo : length l ≥ 2 → encodes amo (sinz l g hdis) l :=
+begin
+  intros hl τ,
+  induction l using strong_induction_on_lists with l ih generalizing g,
+  rcases exists_cons_cons_of_length_ge_two hl with ⟨l₁, l₂, ls, rfl⟩,
+  have hdis' := disjoint_fresh_of_disjoint hdis,
+  have hmem₁ : l₁.flip.var ∈ clause.vars (l₁ :: l₂ :: ls),
+  { simp [flip_var_eq, clause.vars] },
+  have hmemnot₁ : l₁.flip.var ∉ g.stock,
+  { exact set.disjoint_right.mp hdis hmem₁ },
+  have hmem₂ : l₂.flip.var ∈ clause.vars (l₁ :: l₂ :: ls),
+  { simp [flip_var_eq, clause.vars] },
+  have hnmem₁ : g.fresh.1 ∉ clause.vars (l₁ :: l₂ :: ls),
+  { have := set.disjoint_left.mp hdis (fresh_mem_stock g),
+    assumption }, -- TODO coercion is silly
+  have hnmem₂ : g.fresh.2.fresh.1 ∉ clause.vars (l₁ :: l₂ :: ls),
+  { have := fresh_mem_stock g.fresh.2,
+    have := set.disjoint_left.mp hdis (fresh_stock_subset g this),
+    assumption }, -- TODO this too
+  cases ls with l₃ ls,
+  { sorry }, /-split,
+    { intro heval,
+      rw ← amo.eval at heval,
+      cases h₁ : (literal.eval τ l₁),
+      { use assignment.ite (clause.vars [l₁, l₂]) τ all_ff,
+        split,
+        { rw eval_tt_iff_forall_clause_eval_tt,
+          intros c hc,
+          simp [sinz] at hc,
+          rw eval_tt_iff_exists_literal_eval_tt,
+          rcases hc with (rfl | rfl | rfl),
+          { use l₁.flip,
+            rw [ite_pos_lit hmem₁, eval_flip],
+            simp [h₁] },
+          { use Neg g.fresh.1,
+            simp [literal.eval, ite_neg hnmem₁, all_ff] },
+          { use Neg g.fresh.1,
+            simp [literal.eval, ite_neg hnmem₁, all_ff] } },
+        { exact (ite_eqod (clause.vars [l₁, l₂]) τ _).symm } },
+      { use assignment.ite (clause.vars [l₁, l₂]) τ all_tt,
+        split,
+        { rw eval_tt_iff_forall_clause_eval_tt,
+          intros c hc,
+          simp [sinz] at hc,
+          rw eval_tt_iff_exists_literal_eval_tt,
+          rcases hc with (rfl | rfl | rfl),
+          { use Pos g.fresh.1,
+            simp [literal.eval, ite_neg hnmem₁, all_tt] },
+          { use Pos g.fresh.2.fresh.1,
+            simp [literal.eval, ite_neg hnmem₂, all_tt] },
+          { use l₂.flip,
+            have := amo.amo_eval_tt_iff_distinct_eval_ff_of_eval_tt.mp heval,
+            have := this (distinct_double l₁ l₂) h₁,
+            simp [ite_pos_lit hmem₂],
+            rw eval_flip,
+            simp [this] } },
+        { exact (ite_eqod (clause.vars [l₁, l₂]) τ _).symm } } },
+    { rintros ⟨σ, heval, hs⟩,
+    have heq : literal.eval τ l₂ = literal.eval σ l₂,
+    { have : l₂.var ∈ clause.vars [l₁, l₂],
+      { simp [clause.vars] },
+        exact eval_eq_of_eqod_of_var_mem hs this },
+      rw [← amo.eval, eval_eq_amo_of_eqod hs],
+      rw eval_tt_iff_forall_clause_eval_tt at heval,
+      cases h₁ : (literal.eval σ l₁),
+      { rw [eval_cons_neg h₁, amo.eval_singleton] },
+      { have : ∀ (lit₁ lit₂ : literal V), (distinct lit₁ lit₂ [l₁, l₂]) → 
+          lit₁.eval τ = tt → lit₂.eval τ = ff,
+        { intros lit₁ lit₂ hd _,
+          rcases eq_of_distinct_double hd with ⟨rfl, rfl⟩,
+          simp [sinz, clause.eval, eval_flip, literal.eval, h₁] at heval,
+          rcases heval with ⟨hs₁, hs₂, hs₃⟩,
+          simp [hs₁] at hs₃,
+          rw heq,
+          exact hs₃ },
+        rw ← eval_eq_amo_of_eqod hs,
+        exact amo_eval_tt_iff_distinct_eval_ff_of_eval_tt.mpr this } } }, -/
+  { split,
+    { intro heval,
+      rw ← amo.eval at heval,
+      have hless : length (l₂ :: l₃ :: ls) < length (l₁ :: l₂ :: l₃ :: ls), simp,
+      have hlen : length (l₂ :: l₃ :: ls) ≥ 2, dec_trivial,
+      have ihred := ih _ hless hlen hdis',
+      cases h₁ : (literal.eval τ l₁),
+      { sorry }, /- rw eval_cons_neg h₁ at heval,
+        rcases ihred.mp heval with ⟨σ, heval', hs⟩,
+        use assignment.ite (cnf.vars (sinz (l₂ :: l₃ :: ls) g.fresh.2 hdis')) σ 
+            (assignment.ite {l₁.var} τ all_ff),
+        have heval₁ : literal.eval (assignment.ite (cnf.vars (sinz (l₂ :: l₃ :: ls) g.fresh.2 hdis')) σ 
+            (assignment.ite {l₁.var} τ all_ff)) l₁ = ff,
+        { sorry },
+        have heval₂ : (assignment.ite (cnf.vars (sinz (l₂ :: l₃ :: ls) g.fresh.2 hdis')) σ 
+            (assignment.ite {l₁.var} τ all_ff)) g.fresh.1 = ff,
+        { sorry },
+        split,
+        { rw [eval_tt_iff_forall_clause_eval_tt, sinz],
+          intros c hc,
+          rw eval_tt_iff_exists_literal_eval_tt,
+          simp at hc,
+          rcases hc with (rfl | rfl | rfl | hc),
+          { use l₁.flip,
+            simp [eval_flip, heval₁] },
+          { use Neg g.fresh.1,
+            simp [literal.eval, heval₂] },
+          { use Neg g.fresh.1,
+            simp [literal.eval, heval₂] },
+          { rw ← eval_tt_iff_exists_literal_eval_tt,
+            rw eval_tt_iff_forall_clause_eval_tt at heval',
+            rw ← heval' c hc,
+            apply eval_eq_clause_of_eqod,
+            apply eqod_subset (clause_vars_subset_of_vars_of_mem hc),
+            intros v hv,
+            rw ite_pos hv } },
+        { intros v hv,
+          rcases finset.mem_union.mp hv with (hvmem | hvmem),
+          { cases l₁;
+            { simp [literal.flip, literal.eval, var] at h₁ hvmem heval₁ |-,
+              simp [heval₁, hvmem, h₁] } },
+          { rw ite_pos (mem_sinz_vars_of_mem hdis' hlen hvmem),
+            exact hs v hvmem }
+        } }, -/
+      { sorry } },
+      /-
+      { rw eval_cons_pos h₁ at heval,
+        rw amz.eval_tt_iff_forall_eval_ff at heval,
+        use assignment.ite (clause.vars (l₁ :: l₂ :: l₃ :: ls)) τ all_tt,
+        have heval₁ : literal.eval (assignment.ite (clause.vars (l₁ :: l₂ :: l₃ :: ls)) τ all_tt) l₁ = tt,
+        { sorry },
+        have heval₂ : (assignment.ite (clause.vars (l₁ :: l₂ :: l₃ :: ls)) τ all_tt) g.fresh.1 = tt,
+        { sorry },
+        have heval₃ : (assignment.ite (clause.vars (l₁ :: l₂ :: l₃ :: ls)) τ all_tt) g.fresh.2.fresh.1 = tt,
+        { sorry },
+        split,
+        { rw [eval_tt_iff_forall_clause_eval_tt, sinz],
+          intros c hc,
+          simp at hc,
+          rw eval_tt_iff_exists_literal_eval_tt,
+          rcases hc with (rfl | rfl | rfl | hc),
+          { use Pos g.fresh.1,
+            simp [literal.eval, heval₂] },
+          { use Pos g.fresh.2.fresh.1,
+            simp [literal.eval, heval₃] },
+          { use l₂.flip,
+            rw [ite_pos_lit hmem₂, eval_flip],
+            simp [ite_pos_lit hmem₂, eval_flip, heval l₂ (mem_cons_self l₂ _)] },
+          { rw ← amz.eval_tt_iff_forall_eval_ff at heval,
+            have := all_tt_eval_tt_of_amz_eval_tt hdis' hlen heval,
+            rw eval_tt_iff_forall_clause_eval_tt at this,
+            have := this c hc,
+            rcases eval_tt_iff_exists_literal_eval_tt.mp this with ⟨l, hlmem, hle⟩,
+            use [l, hlmem],
+            by_cases hlin : l.var ∈ clause.vars (l₂ :: l₃ :: ls),
+            { rw ite_pos_lit hlin at hle,
+              rw ite_pos_lit (vars_subset_of_vars_cons l₁ (l₂ :: l₃ :: ls) hlin),
+              exact hle },
+            { rw ite_neg_lit hlin at hle,
+              -- show l.var is not equal to l₁.var
+              sorry } } },
+        { intros v hv, rw ite_pos hv } } }, -/
+    {
+      rintros ⟨σ, heval, heqod⟩,
+      rw [sinz, eval_tt_iff_forall_clause_eval_tt] at heval,
+      simp at heval,
+    }
+  }
+end
+-/
 
 end sinz_amo
