src/cardinality/sinz_amk.lean
@@ -1,0 +1,96 @@
+/-
+The Sinz at-most-one encoding.
+
+Authors: Cayden Codel, Jeremy Avigad, Marijn Heule
+Carnegie Mellon University
+-/
+
+import cnf.literal
+import cnf.clause
+import cnf.cnf
+import cnf.encoding
+import cnf.gensym
+
+import cardinality.distinct
+import cardinality.cardinality
+
+import data.list.basic
+import data.nat.basic
+
+variables {V : Type*} [inhabited V] [decidable_eq V]
+
+namespace sinz_amk
+
+open list
+open literal
+open clause
+open cnf
+open assignment
+open encoding
+--open distinct
+open gensym
+--open amo
+
+variables {l : list (literal V)} {lit l₁ l₂ : literal V} {g : gensym V}
+          {τ : assignment V} (hdis : disjoint g.stock (clause.vars l))
+          {c : clause V}
+          {k : nat} (hk : k ≥ 2)
+
+-- Not true, refine later
+lemma a1 {k : nat} : k ≥ 2 → ∀ m, m < k :=
+begin
+  sorry
+end
+
+lemma a2 {k : nat} {l : list V} : k ≥ 2 → length l = k → length l ≥ 2 :=
+begin
+  sorry
+end
+
+lemma disjoint_fresh_of_disjoint : disjoint g.stock (clause.vars (lit :: l)) → 
+  disjoint (g.nfresh k).2.stock (clause.vars l) :=
+begin
+  sorry
+end
+
+def sinz_k {k : nat} (hk : k ≥ 2) : Π (l : list (literal V)), Π (g : gensym V),
+  (disjoint g.stock (clause.vars l)) → cnf V
+| [] _ _ := []
+| [l₁] _ _ := [] -- [l₁.flip, Neg (g.prev)]
+| (l₁ :: l₂ :: ls) g hdis :=
+  --let ⟨ss, g'⟩ := g.nfresh k in
+  have hlen₁ : length (g.nfresh k).1 ≥ 2, from a2 hk (length_list_nfresh g k),
+  have hlen₂ : length ((g.nfresh k).2.nfresh k).1 ≥ 2, 
+    from a2 hk (length_list_nfresh (g.nfresh k).2 k),
+  -- x_i → s_(i, 1)
+  [l₁.flip, Pos (nth_le (g.nfresh k).1 0 (a1 hlen₁ _))] ::
+
+  -- x_(i + 1) → ¬s_(i, k)
+  [l₂.flip, Neg (nth_le (g.nfresh k).1 (k - 1) (a1 hlen₁ _))] ::
+
+  -- s_(i, j) → s_(i + 1, j)
+  (map (λ p : (nat × V), let ⟨i, s⟩ := p in 
+      [Neg s,
+       Pos (nth_le ((g.nfresh k).2.nfresh k).1 i (a1 hlen₂ _))])
+    (enum (g.nfresh k).1))
+  ++
+  (map (λ p : (nat × V), let ⟨i, s⟩ := p in
+      [l₂.flip, Neg s, Pos (nth_le ((g.nfresh k).2.nfresh k).1 (i + 1) (a1 hlen₂ _))])
+      (enum (take (k - 1) (g.nfresh k).1)))
+  ++
+  sinz_k (l₂ :: ls) (g.nfresh k).2 (disjoint_fresh_of_disjoint hdis)
+
+def sinz {k : nat} (hk : k ≥ 2) : Π (l : list (literal V)), Π (g : gensym V),
+  (disjoint g.stock (clause.vars l)) → cnf V
+| l g hdis := (sinz_k hk l g hdis) ++ 
+              -- ¬s_(1, j) for j > 1
+              map (λ s, [Neg s]) (g.nfresh k).1.tail
+
+/-
+    [l₁.flip, Pos (g.fresh.1)] :: 
+    [Neg g.fresh.1, Pos g.fresh.2.fresh.1] ::
+    [Neg g.fresh.1, l₂.flip] ::
+    (sinz (l₂ :: ls) g.fresh.2 (disjoint_fresh_of_disjoint hdis))
+-/
+
+end sinz_amk
